Simplification finished, up to trace equiv

theories/Local.v
@@ -11,49 +11,56 @@ Require Import MPST.LNVar.
 Require Import MPST.Actions.
 
 Section Syntax.
+
+  Inductive l_act := l_send | l_recv.
+
+  Definition eq_lact a b :=
+    match a, b with
+    | l_send, l_send
+    | l_recv, l_recv => true
+    | _, _ => false
+    end.
+
+  Lemma lact_eqP : Equality.axiom eq_lact.
+  Proof. by rewrite /Equality.axiom => [[] []/=]; constructor. Qed.
+
+  Definition lact_eqMixin := EqMixin lact_eqP.
+  Canonical lact_eqType := Eval hnf in EqType l_act lact_eqMixin.
+
   Inductive l_ty :=
   | l_end
   | l_var (v : rvar)
   | l_rec (L : l_ty)
-  | l_send (r : role) (t : mty) (L : l_ty)
-  | l_recv (r : role) (t : mty) (L : l_ty)
-  | l_brn (r : role) (K : seq (lbl * l_ty))
-  | l_sel (r : role) (K : seq (lbl * l_ty)).
+  | l_msg (a : l_act) (r : role) (Ks : seq (lbl * (mty * l_ty)))
+  .
 
   Notation lfv a := (l_var (Rvar.fv a)).
   Notation lbv n := (l_var (Rvar.bv n)).
+
+  Open Scope mpst_scope.
 
   Lemma lty_ind :
     forall (P : l_ty -> Prop),
       P l_end ->
       (forall v, P (l_var v)) ->
       (forall G, P G -> P (l_rec G)) ->
-      (forall r t G, P G -> P (l_send r t G)) ->
-      (forall r t G, P G -> P (l_recv r t G)) ->
-      (forall p K, Forall (fun lL => P lL.2) K -> P (l_brn p K)) ->
-      (forall p K, Forall (fun lL => P lL.2) K -> P (l_sel p K)) ->
+      (forall a p Ks, Forall (fun K => P K.cnt) Ks -> P (l_msg a p Ks)) ->
       forall l : l_ty, P l.
   Proof.
-    move => P P_end P_var P_rec P_send P_recv P_brn P_sel.
-    fix Ih 1; case=>[|v|L|r t L|r t L|r K|r K].
+    move => P P_end P_var P_rec P_msg.
+    fix Ih 1; case=>[|v|L|a r K].
     + by apply: P_end.
     + by apply: P_var.
     + by apply: P_rec.
-    + by apply: P_send.
-    + by apply: P_recv.
-    + by apply: P_brn; elim: K.
-    + by apply: P_sel; elim: K.
+    + by apply: P_msg; elim: K.
   Qed.
 
   Fixpoint depth_lty L :=
     match L with
     | l_end
     | l_var _ => 0
-    | l_rec L
-    | l_recv _ _ L
-    | l_send _ _ L => (depth_lty L).+1
-    | l_sel _ K
-    | l_brn _ K  => (maximum [seq depth_lty l.2 | l <- K]).+1
+    | l_rec L => (depth_lty L).+1
+    | l_msg _ _ Ks => (maximum [seq depth_lty K.cnt | K <- Ks]).+1
     end.
 
   Fixpoint eq_lty x y :=
@@ -61,58 +68,43 @@ Section Syntax.
     | l_end, l_end => true
     | l_var x, l_var y => x == y
     | l_rec x, l_rec y => eq_lty x y
-    | l_recv r1 t1 L1, l_recv r2 t2 L2
-    | l_send r1 t1 L1, l_send r2 t2 L2
-      => (r1 == r2) && (t1 == t2) && eq_lty L1 L2
-    | l_sel r1 K1, l_sel r2 K2
-    | l_brn r1 K1, l_brn r2 K2
-      => (r1 == r2)
-           && (fix eqK K1 K2 :=
-                 match K1, K2 with
+    | l_msg a1 r1 Ks1, l_msg a2 r2 Ks2
+      => (a1 == a2) && (r1 == r2)
+           && (fix eqK Ks1 Ks2 :=
+                 match Ks1, Ks2 with
                  | [::], [::] => true
-                 | (l1, L1)::K1, (l2, L2)::K2 =>
-                   (l1 == l2) && eq_lty L1 L2 && eqK K1 K2
+                 | K1::Ks1, K2::Ks2 =>
+                   (K1.lbl == K2.lbl)
+                     && (K1.mty == K2.mty)
+                     && eq_lty K1.cnt K2.cnt
+                     && eqK Ks1 Ks2
                  | _, _ => false
-                 end) K1 K2
+                 end) Ks1 Ks2
            (* all2 (fun l r => (l.1 == r.1) && eq_lty l.2 r.2) K1 K2 *)
     | _, _ => false
     end.
 
-  Definition eq_lalt (l r : lbl * l_ty) := (l.1 == r.1) && eq_lty l.2 r.2.
+  Definition eq_lalt (l r : lbl * (mty * l_ty)) :=
+    (l.lbl == r.lbl) && (l.mty == r.mty) && eq_lty l.cnt r.cnt.
 
-  Lemma eqbrn_all r1 r2 K1 K2 :
-    eq_lty (l_brn r1 K1) (l_brn r2 K2) = (r1 == r2) && all2 eq_lalt K1 K2.
+  Lemma eqmsg_all a1 a2 r1 r2 K1 K2 :
+    eq_lty (l_msg a1 r1 K1) (l_msg a2 r2 K2) =
+    (a1 == a2) && (r1 == r2) && all2 eq_lalt K1 K2.
   Proof.
-    rewrite /=; case: eqP=>///= _; move: K1 K2 {r1 r2}.
-    by elim=>//[[l1 L1] K1] Ih; case=>//[[l2 L2] K2]/=; rewrite Ih.
-  Qed.
-
-  Lemma eqsel_all r1 r2 K1 K2 :
-    eq_lty (l_sel r1 K1) (l_sel r2 K2) = (r1 == r2) && all2 eq_lalt K1 K2.
-  Proof.
-    rewrite /=; case: eqP=>///= _; move: K1 K2 {r1 r2}.
+    rewrite /=; do 2 (case: eqP=>///= _); move: K1 K2 {r1 r2 a1 a2}.
     by elim=>//[[l1 L1] K1] Ih; case=>//[[l2 L2] K2]/=; rewrite Ih.
   Qed.
 
   Lemma lty_eqP : Equality.axiom eq_lty.
   Proof.
     rewrite /Equality.axiom; fix Ih 1 => x y.
-    case: x => [|v|L|r t L|r t L|r K|r K];
-       case: y =>[|v'|L'|r' t' L'|r' t' L'|r' K'|r' K']; try (by constructor).
+    case: x => [|v|L|a r K]; case: y =>[|v'|L'|a' r' K']; try (by constructor).
     + by rewrite /eq_lty; case: eqP=>[->|F]; constructor=>//[[/F]].
     + by rewrite /=; case: Ih=>[->|F]; constructor=>//[[/F]].
-    + rewrite /=; do 2 (case: eqP=>[->|F];[|constructor=>[[/F]]//]).
-      by case: Ih=>[->|F];constructor=>//[[/F]].
-    + rewrite /=; do 2 (case: eqP=>[->|F];[|constructor=>[[/F]]//]).
-      by case: Ih=>[->|F];constructor=>//[[/F]].
-    + rewrite eqbrn_all; case: eqP=>[<-|F];[|constructor=>[[/F]]//];move:K'=>/=.
-      elim: K=>[|[l L] K IhK]; case=>[|[l' L']K']/=; try (by constructor).
-      rewrite {1}/eq_lalt/=; case: eqP=>[<-|F];[|constructor=>[[/F]]//].
-      case: Ih=>[<-|F];[|constructor=>[[/F]]//].
-      by case: IhK=>[[]<-|F]; constructor=>//[[]]H; apply: F; rewrite H.
-    + rewrite eqsel_all; case: eqP=>[<-|F];[|constructor=>[[/F]]//];move:K'=>/=.
-      elim: K=>[|[l L] K IhK]; case=>[|[l' L']K']/=; try (by constructor).
-      rewrite {1}/eq_lalt/=; case: eqP=>[<-|F];[|constructor=>[[/F]]//].
+    + rewrite eqmsg_all; do 2 (case: eqP=>[<-|F]/=;[|constructor=>[[/F]]//]).
+      elim: K K'=>[|[l [t L]] K IhK];
+        case=>[|[l' [t' L']]K']/=; try (by constructor).
+      rewrite {1}/eq_lalt/=; do 2 (case: eqP=>[<-|F];[|constructor=>[[/F]]//]).
       case: Ih=>[<-|F];[|constructor=>[[/F]]//].
       by case: IhK=>[[]<-|F]; constructor=>//[[]]H; apply: F; rewrite H.
   Qed.
@@ -125,10 +117,8 @@ Section Syntax.
     | l_end => L1
     | l_var v => Rvar.open l_var d L2 v
     | l_rec L => l_rec (l_open d.+1 L2 L)
-    | l_send p t L => l_send p t (l_open d L2 L)
-    | l_recv p t L => l_recv p t (l_open d L2 L)
-    | l_brn p K => l_brn p [seq (lL.1, l_open d L2 lL.2) | lL <- K]
-    | l_sel p K => l_sel p [seq (lL.1, l_open d L2 lL.2) | lL <- K]
+    | l_msg a p Ks =>
+      l_msg a p [seq (K.lbl, (K.mty, l_open d L2 K.cnt)) | K <- Ks]
     end.
   Notation "{ k '~>' v } L":= (l_open k v L) (at level 30, right associativity).
   Notation "L '^' v":= (l_open 0 (lfv v) L) (at level 30, right associativity).
@@ -138,10 +128,8 @@ Section Syntax.
     | l_end => L1
     | l_var lv => l_var (Rvar.close v d lv)
     | l_rec L => l_rec (l_close v d.+1 L)
-    | l_send p t L => l_send p t (l_close v d L)
-    | l_recv p t L => l_recv p t (l_close v d L)
-    | l_brn p K => l_brn p [seq (lL.1, l_close v d lL.2) | lL <- K]
-    | l_sel p K => l_sel p [seq (lL.1, l_close v d lL.2) | lL <- K]
+    | l_msg a p Ks =>
+      l_msg a p [seq (K.lbl, (K.mty, l_close v d K.cnt)) | K <- Ks]
     end.
   Notation "{ k '<~' v } L":= (l_close v k L) (at level 30, right associativity).
 
@@ -157,15 +145,18 @@ Section Syntax.
     zip (unzip1 K) [seq f x | x <- unzip2 K] = [seq (x.1, f x.2) | x <- K].
   Proof. by rewrite unzip2_lift (unzip1_map2 f) zip_unzip. Qed.
 
-  Lemma lclose_brn_zip v d p K :
-    l_close v d (l_brn p K)
-    = l_brn p (zip (unzip1 K) [seq l_close v d x | x <- unzip2 K]).
+
+  (*
+  Lemma lclose_send_zip v d p K :
+    l_close v d (l_send p K)
+    = l_send p (zip (unzip1 K) (zip (unzip1 (unzip2 K)) [seq l_close v d x | x <- unzip2 (unzip2 K)])).
   Proof. by rewrite /= unzip2_lift (unzip1_map2 (l_close v d)) zip_unzip. Qed.
 
   Lemma lclose_sel_zip v d p K :
     l_close v d (l_sel p K)
     = l_sel p (zip (unzip1 K) [seq l_close v d x | x <- unzip2 K]).
   Proof. by rewrite /= unzip2_lift (unzip1_map2 (l_close v d)) zip_unzip. Qed.
+   *)
 
   Definition fsetUs (K : choiceType) : seq {fset K} -> {fset K}
     := foldl fsetU fset0.
@@ -181,11 +172,8 @@ Section Syntax.
     match L with
     | l_end => fset0
     | l_var v => Rvar.fvar v
-    | l_rec L
-    | l_recv _ _ L
-    | l_send _ _ L => l_fvar L
-    | l_sel _ K
-    | l_brn _ K => fsetUs [seq l_fvar lL.2 | lL <- K]
+    | l_rec L => l_fvar L
+    | l_msg _ _ K => fsetUs [seq l_fvar lL.cnt | lL <- K]
     end.
 
   Fixpoint l_fbvar (d : nat) (L : l_ty) : {fset nat} :=
@@ -193,23 +181,17 @@ Section Syntax.
     | l_end => fset0
     | l_var v => Rvar.fbvar d v
     | l_rec L => l_fbvar d.+1 L
-    | l_recv _ _ L
-    | l_send _ _ L => l_fbvar d L
-    | l_sel _ K
-    | l_brn _ K => fsetUs [seq l_fbvar d lL.2 | lL <- K]
+    | l_msg _ _ K => fsetUs [seq l_fbvar d lL.cnt | lL <- K]
     end.
 
   Lemma l_open_close X L n : X \notin l_fvar L -> {n <~ X}{n ~> lfv X}L = L.
   Proof.
-    elim/lty_ind: L n=>[|v|L Ih|r t L Ih|r t L Ih|r K Ih|r K Ih] n /=Fv//;
+    elim/lty_ind: L n=>[|v|L Ih|a r K Ih] n /=Fv//;
       try (by rewrite Ih).
     + by move: Fv; rewrite Rvar.open_fun/= =>H; rewrite Rvar.open_close.
     + move: Ih=>/Fa_lift/(_ n)-Ih; move: Fv => /notin_unions/Fa_map-Fv.
       move: (Fa_app (Fa_conj Ih Fv)) => {Ih Fv}Ih; rewrite -map_comp /comp/=.
-      by elim: K Ih=>// [[l L] K Ih/= [-> /Ih-[->]]].
-    + move: Ih=>/Fa_lift/(_ n)-Ih; move: Fv => /notin_unions/Fa_map-Fv.
-      move: (Fa_app (Fa_conj Ih Fv)) => {Ih Fv}Ih; rewrite -map_comp /comp/=.
-      by elim: K Ih=>// [[l L] K Ih/= [-> /Ih-[->]]].
+      by elim: K Ih=>// [[l [t L]] K Ih/= [-> /Ih-[->]]].
   Qed.
 
   Lemma l_close_open n X L : n \notin l_fbvar 0 L -> {n ~> lfv X}{n <~ X}L = L.
@@ -217,16 +199,10 @@ Section Syntax.
     move: {1 3}n (add0n n)=>n0; elim/lty_ind: L 0 n =>///=.
     - by move=>v n n1;rewrite addnC Rvar.open_fun=><-H;rewrite Rvar.close_open.
     - by move=>G Ih n n1 Eq/= H; rewrite (Ih n.+1 n1.+1) // -Eq.
-    - by move=> r t G Ih n n1 Eq/= H; rewrite (Ih n n1).
-    - by move=> r t G Ih n n1 Eq/= H; rewrite (Ih n n1).
-    - move=> r K /Fa_lift-Ih n n1 Eq /notin_unions/Fa_map-H.
+    - move=> a r K /Fa_lift-Ih n n1 Eq /notin_unions/Fa_map-H.
       move:Ih=>/(_ n)/Fa_lift/(_ n1)/Fa_lift/(_ Eq)/Fa_conj/( _ H)/Fa_app-Ih{H}.
-      rewrite -map2_zip -unzip1_map2 unzip2_lift /unzip2 -!map_comp /comp/=.
-      by rewrite (Fa_map_eq Ih) zip_unzip.
-    - move=> r K /Fa_lift-Ih n n1 Eq /notin_unions/Fa_map-H.
-      move:Ih=>/(_ n)/Fa_lift/(_ n1)/Fa_lift/(_ Eq)/Fa_conj/( _ H)/Fa_app-Ih{H}.
-      rewrite -map2_zip -unzip1_map2 unzip2_lift /unzip2 -!map_comp /comp/=.
-      by rewrite (Fa_map_eq Ih) zip_unzip.
+      congr l_msg; rewrite -map_comp/comp/=.
+      by elim: K Ih => [// | [l [t L]] K/= IhL [-> /IhL->]].
   Qed.
 
   Lemma l_depth_open L X : depth_lty L = depth_lty (L^X).
@@ -234,11 +210,7 @@ Section Syntax.
     move: 0; elim/lty_ind: L=>/=//.
     + by move=>v n; rewrite Rvar.open_fun.
     + by move=> L Ih n; rewrite (Ih n.+1).
-    + by move=> _ _ L Ih n; rewrite (Ih n).
-    + by move=> _ _ L Ih n; rewrite (Ih n).
-    + move=> _ K Ih n; rewrite -map_comp /comp/=.
-      by move: Ih => /Fa_lift/(_ n)/Fa_map_eq<-.
-    + move=> _ K Ih n; rewrite -map_comp /comp/=.
+    + move=> _ _ K Ih n; rewrite -map_comp /comp/=.
       by move: Ih => /Fa_lift/(_ n)/Fa_map_eq<-.
   Qed.
 
@@ -248,23 +220,15 @@ Section Syntax.
       (forall v, P (l_var v)) ->
       (forall L, (forall X (s : {fset atom}), X \notin s -> P (L ^ X)) ->
                  P (l_rec L)) ->
-      (forall r t L, P L -> P (l_send r t L)) ->
-      (forall r t L, P L -> P (l_recv r t L)) ->
-      (forall p K, (forall l L, (l, L) \in K -> P L) -> P (l_brn p K)) ->
-      (forall p K, (forall l L, (l, L) \in K -> P L) -> P (l_sel p K)) ->
+      (forall a p Ks, (forall K, K \in Ks -> P K.cnt) -> P (l_msg a p Ks)) ->
       forall l : l_ty, P l.
   Proof.
-    move => P P_end P_var P_rec P_send P_recv P_brn P_sel L.
+    move => P P_end P_var P_rec P_msg L.
     move: {-1}(depth_lty L) (leqnn (depth_lty L))=> n; move: n L; elim.
     + by case.
     + move=>n Ih; case=>/=//.
       - by move=>L D; apply:P_rec=>X S _;apply: Ih;rewrite -(l_depth_open L X).
-      - by move=> r t L D; apply: P_send; apply: Ih.
-      - by move=> r t L D; apply: P_recv; apply: Ih.
-      - move=> r K D;apply: P_brn=>l L /(map_f (fun X => depth_lty X.2)).
-        move=>/in_maximum_leq-/=dG; move: (leq_trans dG D)=>{dG} {D}.
-        by apply: Ih.
-      - move=> r K D;apply: P_sel=>l L /(map_f (fun X => depth_lty X.2)).
+      - move=> a r Ks D;apply: P_msg=>K /(map_f (fun X => depth_lty X.cnt)).
         move=>/in_maximum_leq-/=dG; move: (leq_trans dG D)=>{dG} {D}.
         by apply: Ih.
   Qed.
@@ -276,67 +240,50 @@ Section Session.
   | s_end
   | s_var (v : rvar)
   | s_rec (S : s_ty)
-  | s_send (t : mty) (S : s_ty)
-  | s_recv (t : mty) (L : s_ty)
-  | s_brn (K : seq (lbl * s_ty))
-  | s_sel (K : seq (lbl * s_ty)).
+  | s_msg (a: l_act) (K : seq (lbl * (mty * s_ty))).
+
+  Open Scope mpst_scope.
 
   Fixpoint eq_sty x y :=
     match x, y with
     | s_end, s_end => true
     | s_var x, s_var y => x == y
     | s_rec x, s_rec y => eq_sty x y
-    | s_recv t1 S1, s_recv t2 S2
-    | s_send t1 S1, s_send t2 S2
-      => (t1 == t2) && eq_sty S1 S2
-    | s_sel K1, s_sel K2
-    | s_brn K1, s_brn K2
-      => (fix eqK K1 K2 :=
-            match K1, K2 with
-            | [::], [::] => true
-            | (l1, S1)::K1, (l2, S2)::K2 =>
-              (l1 == l2) && eq_sty S1 S2 && eqK K1 K2
-            | _, _ => false
-            end) K1 K2
-           (* all2 (fun l r => (l.1 == r.1) && eq_lty l.2 r.2) K1 K2 *)
+    | s_msg a1 Ks1, s_msg a2 Ks2
+      => (a1 == a2)
+           && (fix eqK Ks1 Ks2 :=
+                 match Ks1, Ks2 with
+                 | [::], [::] => true
+                 | K1::Ks1, K2::Ks2 =>
+                   (K1.lbl == K2.lbl)
+                     && (K1.mty == K2.mty)
+                     && eq_sty K1.cnt K2.cnt && eqK Ks1 Ks2
+                 | _, _ => false
+                 end) Ks1 Ks2
+    (* all2 (fun l r => (l.1 == r.1) && eq_lty l.2 r.2) K1 K2 *)
     | _, _ => false
     end.
 
-  Definition eq_salt (l r : lbl * s_ty) := (l.1 == r.1) && eq_sty l.2 r.2.
+  Definition eq_salt (l r : lbl * (mty * s_ty)) :=
+    (l.lbl == r.lbl) && (l.mty == r.mty) && eq_sty l.cnt r.cnt.
 
-  Lemma eq_sbrn_all K1 K2 :
-    eq_sty (s_brn K1) (s_brn K2) = all2 eq_salt K1 K2.
+  Lemma eq_smsg_all a1 a2 K1 K2 :
+    eq_sty (s_msg a1 K1) (s_msg a2 K2) = (a1 == a2) && all2 eq_salt K1 K2.
   Proof.
-    rewrite /=; move: K1 K2.
-    by elim=>//[[l1 L1] K1] Ih; case=>//[[l2 L2] K2]/=; rewrite Ih.
-  Qed.
-
-  Lemma eq_ssel_all K1 K2 :
-    eq_sty (s_sel K1) (s_sel K2) = all2 eq_salt K1 K2.
-  Proof.
-    rewrite /=; move: K1 K2.
-    by elim=>//[[l1 L1] K1] Ih; case=>//[[l2 L2] K2]/=; rewrite Ih.
+    rewrite /=; case: eqP=>[/=_{a1 a2}|//]; move: K1 K2.
+    by elim=>//[[l1 [t1 L1]] K1] Ih; case=>//[[l2 [t2 L2]] K2]/=; rewrite Ih.
   Qed.
 
   Lemma sty_eqP : Equality.axiom eq_sty.
   Proof.
     rewrite /Equality.axiom; fix Ih 1 => x y.
-    case: x => [|v|L|t L|t L|K|K];
-       case: y =>[|v'|L'|t' L'|t' L'|K'|K']; try (by constructor).
+    case: x => [|v|L|a K];
+       case: y =>[|v'|L'|a' K']; try (by constructor).
     + by rewrite /eq_sty; case: eqP=>[->|F]; constructor=>//[[/F]].
     + by rewrite /=; case: Ih=>[->|F]; constructor=>//[[/F]].
-    + rewrite /=; case: eqP=>[->|F];[|constructor=>[[/F]]//].
-      by case: Ih=>[->|F];constructor=>//[[/F]].
-    + rewrite /=; case: eqP=>[->|F];[|constructor=>[[/F]]//].
-      by case: Ih=>[->|F];constructor=>//[[/F]].
-    + rewrite eq_sbrn_all; move: K'.
-      elim: K=>[|[l L] K IhK]; case=>[|[l' L']K']/=; try (by constructor).
-      rewrite {1}/eq_salt/=; case: eqP=>[<-|F];[|constructor=>[[/F]]//].
-      case: Ih=>[<-|F];[|constructor=>[[/F]]//].
-      by case: IhK=>[[]<-|F]; constructor=>//[[]]H; apply: F; rewrite H.
-    + rewrite eq_ssel_all; move:K'=>/=.
-      elim: K=>[|[l L] K IhK]; case=>[|[l' L']K']/=; try (by constructor).
-      rewrite {1}/eq_salt/=; case: eqP=>[<-|F];[|constructor=>[[/F]]//].
+    + rewrite eq_smsg_all/=; case: eqP=>[<-{a'}|F]/=; [|by constructor=>[[/F]]].
+      elim: K K'=>[|[l [t L]] K IhK]; case=>[|[l' [t' L']]K']/=; try (by constructor).
+      rewrite {1}/eq_salt/=; do 2 (case: eqP=>[<-|F];[|constructor=>[[/F]]//]).
       case: Ih=>[<-|F];[|constructor=>[[/F]]//].
       by case: IhK=>[[]<-|F]; constructor=>//[[]]H; apply: F; rewrite H.
   Qed.
@@ -349,10 +296,7 @@ Section Session.
     | s_end => S1
     | s_var v => Rvar.open s_var d S2 v
     | s_rec s => s_rec (s_open d.+1 S2 s)
-    | s_send t s => s_send t (s_open d S2 s)
-    | s_recv t s => s_recv t (s_open d S2 s)
-    | s_brn K => s_brn [seq (lS.1, s_open d S2 lS.2) | lS <- K]
-    | s_sel K => s_sel [seq (lS.1, s_open d S2 lS.2) | lS <- K]
+    | s_msg a K => s_msg a [seq (lS.lbl, (lS.mty, s_open d S2 lS.cnt)) | lS <- K]
     end.
   Notation sfv a := (s_var (Rvar.fv a)).
   Notation sbv n := (s_var (Rvar.bv n)).
@@ -364,10 +308,7 @@ Section Session.
     | s_end => L1
     | s_var lv => s_var (Rvar.close v d lv)
     | s_rec L => s_rec (s_close v d.+1 L)
-    | s_send t L => s_send t (s_close v d L)
-    | s_recv t L => s_recv t (s_close v d L)
-    | s_brn K => s_brn [seq (lL.1, s_close v d lL.2) | lL <- K]
-    | s_sel K => s_sel [seq (lL.1, s_close v d lL.2) | lL <- K]
+    | s_msg a K => s_msg a [seq (lL.lbl, (lL.mty, s_close v d lL.cnt)) | lL <- K]
     end.
   Notation "{ k '<~' v } L":= (s_close v k L) (at level 30, right associativity).
 
@@ -375,11 +316,8 @@ Section Session.
     match L with
     | s_end => fset0
     | s_var v => Rvar.fvar v
-    | s_rec L
-    | s_recv _ L
-    | s_send _ L => s_fvar L
-    | s_sel K
-    | s_brn K => fsetUs [seq s_fvar lL.2 | lL <- K]
+    | s_rec L => s_fvar L
+    | s_msg _ K => fsetUs [seq s_fvar lL.cnt | lL <- K]
     end.
 
   Fixpoint s_fbvar (d : nat) (L : s_ty) : {fset nat} :=
@@ -387,10 +325,7 @@ Section Session.
     | s_end => fset0
     | s_var v => Rvar.fbvar d v
     | s_rec L => s_fbvar d.+1 L
-    | s_recv _ L
-    | s_send _ L => s_fbvar d L
-    | s_sel K
-    | s_brn K => fsetUs [seq s_fbvar d lL.2 | lL <- K]
+    | s_msg _ K => fsetUs [seq s_fbvar d lL.cnt | lL <- K]
     end.
 
   Lemma sty_ind :
@@ -398,34 +333,25 @@ Section Session.
       P s_end ->
       (forall v, P (s_var v)) ->
       (forall s, P s -> P (s_rec s)) ->
-      (forall t s, P s -> P (s_send t s)) ->
-      (forall t s, P s -> P (s_recv t s)) ->
-      (forall K, Forall (fun lS => P lS.2) K -> P (s_brn K)) ->
-      (forall K, Forall (fun lS => P lS.2) K -> P (s_sel K)) ->
+      (forall a K, Forall (fun lS => P lS.cnt) K -> P (s_msg a K)) ->
       forall s : s_ty, P s.
   Proof.
-    move => P P_end P_var P_rec P_send P_recv P_brn P_sel.
-    fix Ih 1; case=>[|v|L|t L|t L|K|K].
+    move => P P_end P_var P_rec P_msg.
+    fix Ih 1; case=>[|v|L|a K].
     + by apply: P_end.
     + by apply: P_var.
     + by apply: P_rec.
-    + by apply: P_send.
-    + by apply: P_recv.
-    + by apply: P_brn; elim: K.
-    + by apply: P_sel; elim: K.
+    + by apply: P_msg; elim: K.
   Qed.
 
   Lemma s_open_close X L n : X \notin s_fvar L -> {n <~ X}{n ~> sfv X}L = L.
   Proof.
-    elim/sty_ind: L n=>[|v|L Ih|t L Ih|t L Ih|K Ih|K Ih] n /=Fv//;
+    elim/sty_ind: L n=>[|v|L Ih|a K Ih] n /=Fv//;
       try (by rewrite Ih).
     + by move: Fv; rewrite Rvar.open_fun/= =>H; rewrite Rvar.open_close.
     + move: Ih=>/Fa_lift/(_ n)-Ih; move: Fv => /notin_unions/Fa_map-Fv.
       move: (Fa_app (Fa_conj Ih Fv)) => {Ih Fv}Ih; rewrite -map_comp /comp/=.
-      by elim: K Ih=>// [[l L] K Ih/= [-> /Ih-[->]]].
-    + move: Ih=>/Fa_lift/(_ n)-Ih; move: Fv => /notin_unions/Fa_map-Fv.
-      move: (Fa_app (Fa_conj Ih Fv)) => {Ih Fv}Ih; rewrite -map_comp /comp/=.
-      by elim: K Ih=>// [[l L] K Ih/= [-> /Ih-[->]]].
+      by elim: K Ih=>// [[l [t L]] K Ih/= [-> /Ih-[->]]].
   Qed.
 
   Lemma s_close_open n X L : n \notin s_fbvar 0 L -> {n ~> sfv X}{n <~ X}L = L.
@@ -433,27 +359,18 @@ Section Session.
     move: {1 3}n (add0n n)=>n0; elim/sty_ind: L 0 n =>///=.
     - by move=>v n n1;rewrite addnC Rvar.open_fun=><-H;rewrite Rvar.close_open.
     - by move=>G Ih n n1 Eq/= H; rewrite (Ih n.+1 n1.+1) // -Eq.
-    - by move=> t G Ih n n1 Eq/= H; rewrite (Ih n n1).
-    - by move=> t G Ih n n1 Eq/= H; rewrite (Ih n n1).
-    - move=> K /Fa_lift-Ih n n1 Eq /notin_unions/Fa_map-H.
+    - move=> a K /Fa_lift-Ih n n1 Eq /notin_unions/Fa_map-H.
       move:Ih=>/(_ n)/Fa_lift/(_ n1)/Fa_lift/(_ Eq)/Fa_conj/( _ H)/Fa_app-Ih{H}.
-      rewrite -map2_zip -unzip1_map2 unzip2_lift /unzip2 -!map_comp /comp/=.
-      by rewrite (Fa_map_eq Ih) zip_unzip.
-    - move=> K /Fa_lift-Ih n n1 Eq /notin_unions/Fa_map-H.
-      move:Ih=>/(_ n)/Fa_lift/(_ n1)/Fa_lift/(_ Eq)/Fa_conj/( _ H)/Fa_app-Ih{H}.
-      rewrite -map2_zip -unzip1_map2 unzip2_lift /unzip2 -!map_comp /comp/=.
-      by rewrite (Fa_map_eq Ih) zip_unzip.
+      congr s_msg; rewrite -map_comp/comp/=; elim: K Ih=>[//|[l[t S]] K Ih /=].
+      by move=>[->/Ih->].
   Qed.
 
   Fixpoint depth_sty L :=
     match L with
     | s_end
     | s_var _ => 0
-    | s_rec L
-    | s_recv _ L
-    | s_send _ L => (depth_sty L).+1
-    | s_sel K
-    | s_brn K  => (maximum [seq depth_sty l.2 | l <- K]).+1
+    | s_rec L => (depth_sty L).+1
+    | s_msg _ K  => (maximum [seq depth_sty l.cnt | l <- K]).+1
     end.
 
   Lemma s_depth_open L X : depth_sty L = depth_sty (L^X).
@@ -461,11 +378,7 @@ Section Session.
     move: 0; elim/sty_ind: L=>/=//.
     + by move=>v n; rewrite Rvar.open_fun.
     + by move=> L Ih n; rewrite (Ih n.+1).
-    + by move=> _ L Ih n; rewrite (Ih n).
-    + by move=> _ L Ih n; rewrite (Ih n).
-    + move=> K Ih n; rewrite -map_comp /comp/=.
-      by move: Ih => /Fa_lift/(_ n)/Fa_map_eq<-.
-    + move=> K Ih n; rewrite -map_comp /comp/=.
+    + move=> a K Ih n; rewrite -map_comp /comp/=.
       by move: Ih => /Fa_lift/(_ n)/Fa_map_eq<-.
   Qed.
 
@@ -475,93 +388,67 @@ Section Session.
       (forall v, P (s_var v)) ->
       (forall s, (forall X (A : {fset atom}), X \notin A -> P (s ^ X)) ->
                  P (s_rec s)) ->
-      (forall t s, P s -> P (s_send t s)) ->
-      (forall t s, P s -> P (s_recv t s)) ->
-      (forall K, (forall l s, (l, s) \in K -> P s) -> P (s_brn K)) ->
-      (forall K, (forall l s, (l, s) \in K -> P s) -> P (s_sel K)) ->
+      (forall a Ks, (forall K, K \in Ks -> P K.cnt) -> P (s_msg a Ks)) ->
       forall s : s_ty, P s.
   Proof.
-    move => P P_end P_var P_rec P_send P_recv P_brn P_sel L.
+    move => P P_end P_var P_rec P_msg L.
     move: {-1}(depth_sty L) (leqnn (depth_sty L))=> n; move: n L; elim.
     + by case.
     + move=>n Ih; case=>/=//.
       - by move=>L D; apply:P_rec=>X S _;apply: Ih;rewrite -(s_depth_open L X).
-      - by move=> t L D; apply: P_send; apply: Ih.
-      - by move=> t L D; apply: P_recv; apply: Ih.
-      - move=> K D;apply: P_brn=>l L /(map_f (fun X => depth_sty X.2)).
-        move=>/in_maximum_leq-/=dG; move: (leq_trans dG D)=>{dG} {D}.
-        by apply: Ih.
-      - move=> K D;apply: P_sel=>l L /(map_f (fun X => depth_sty X.2)).
+      - move=> a K D;apply: P_msg =>L /(map_f (fun X => depth_sty X.cnt)).
         move=>/in_maximum_leq-/=dG; move: (leq_trans dG D)=>{dG} {D}.
         by apply: Ih.
   Qed.
 
-  Definition pmerge (s : option s_ty) (l : lbl * s_ty) :=
-    match s, l with
-    | None, _ => None
-    | Some s, (_, s') => if s == s' then Some s else None
+  Definition pmerge (s : option s_ty) (l : lbl * (mty * s_ty)) :=
+    match s with
+    | None => None
+    | Some s => if s == l.cnt then Some s else None
     end.
 
-  Definition partial_merge (l : seq (lbl * s_ty)) :=
+  Definition partial_merge (l : seq (lbl * (mty * s_ty))) :=
     match l with
     | [::] => None
-    | h :: t => foldl pmerge (Some h.2) t
+    | h :: t => foldl pmerge (Some h.cnt) t
     end.
 
-  Definition ms_send t L :=
-    match L with
-    | Some L => Some (s_send t L)
-    | None => None
-    end.
-
-  Definition ms_recv t L :=
-    match L with
-    | Some L => Some (s_recv t L)
-    | None => None
-    end.
-
-  Fixpoint merge (A: eqType) (oL : A) (K : seq (lbl * option A)) :=
+  Fixpoint merge (A: eqType) (oL : A) (K : seq (option A)) :=
     match K with
     | [::] => Some oL
-    | h::t => if h.2 == Some oL then merge oL t
+    | h::t => if h == Some oL then merge oL t
               else None
     end.
 
-  Definition merge_all (A : eqType) (K : seq (lbl * option A)) :=
+  Definition merge_all (A : eqType) (K : seq (option A)) :=
     match K with
     | [::] => None
     | (h :: t) =>
-      match h.2 with
+      match h with
       | Some o => merge o t
       | None => None
       end
     end.
 
-  Fixpoint flatten A (L : seq (lbl * option A)) :=
+  Fixpoint flatten A (L : seq (lbl * (mty * option A))) :=
     match L with
     | [::] => Some [::]
-    | h :: t => match h.2, flatten t with
+    | h :: t => match h.cnt, flatten t with
                 | None, _ => None
                 | _, None => None
-                | Some s, Some t => Some ((h.1, s) :: t)
+                | Some s, Some t => Some ((h.lbl, (h.mty, s)) :: t)
                 end
     end.
 
-  Definition flat_alts A (L : seq (lbl * option A)) :=
+  Definition flat_alts A (L : seq (lbl * (mty * option A))) :=
     match L with
     | [::] => None
     | _ => flatten L
     end.
 
-  Definition ms_sel L :=
+  Definition ms_msg a L :=
     match flat_alts L with
-    | Some L => Some (s_sel L)
-    | None => None
-    end.
-
-  Definition ms_brn L :=
-    match flat_alts L with
-    | Some L => Some (s_brn L)
+    | Some L => Some (s_msg a L)
     | None => None
     end.
 
@@ -578,16 +465,15 @@ Section Session.
     | l_rec L =>
       let: s := partial_proj L r in
       if s == Some (sbv 0) then Some s_end else ms_rec s
-    | l_recv p t L =>
-      if p == r then ms_recv t (partial_proj L r) else partial_proj L r
-    | l_send p t L =>
-      if p == r then ms_send t (partial_proj L r) else partial_proj L r
-    | l_sel p K =>
-      if p == r then ms_sel [seq (X.1, partial_proj X.2 r) | X <- K]
-      else merge_all [seq (X.1, partial_proj X.2 r) | X <- K]
-    | l_brn p K  =>
-      if p == r then ms_brn [seq (X.1, partial_proj X.2 r) | X <- K]
-      else merge_all [seq (X.1, partial_proj X.2 r) | X <- K]
+    | l_msg a p K =>
+      if p == r then ms_msg a [seq (X.lbl, (X.mty, partial_proj X.cnt r)) | X <- K]
+      else merge_all [seq partial_proj X.cnt r | X <- K]
+    end.
+
+  Definition dual_act a :=
+    match a with
+    | l_send => l_recv
+    | l_recv => l_send
     end.
 
   Fixpoint dual (L : s_ty) : s_ty :=
@@ -595,19 +481,17 @@ Section Session.
     | s_end => s_end
     | s_var v => s_var v
     | s_rec s => s_rec (dual s)
-    | s_send t L =>  s_recv t (dual L)
-    | s_recv t L =>  s_send t (dual L)
-    | s_brn K => s_sel [seq (x.1, dual x.2) | x <- K]
-    | s_sel K => s_brn [seq (x.1, dual x.2) | x <- K]
+    | s_msg a K => s_msg (dual_act a) [seq (x.lbl, (x.mty, dual x.cnt)) | x <- K]
     end.
+
+  Lemma dual_actK a : dual_act (dual_act a) = a.
+  Proof. by case: a. Qed.
 
   Lemma dualK s : dual (dual s) = s.
   Proof.
-    elim/sty_ind: s=>[|v|s Ih|t s Ih| t s Ih|K Ih|K Ih]//; try (by rewrite /=Ih).
-    - rewrite /= -map_comp /comp/=.
-      by elim: K Ih=>[//|[l s] K Ihl /= [-> /Ihl-[->]]].
-    - rewrite /= -map_comp /comp/=.
-      by elim: K Ih=>[//|[l s] K Ihl /= [-> /Ihl-[->]]].
+    elim/sty_ind: s=>[|v|s Ih|a K Ih]//; try (by rewrite /=Ih).
+    - rewrite /= -map_comp /comp/= dual_actK.
+      by elim: K Ih=>[//|[l [t s]] K Ihl /= [-> /Ihl-[->]]].
   Qed.
 
   Definition is_dual (s1 s2 : s_ty) : bool := s1 == dual s2.
@@ -640,19 +524,19 @@ Section Semantics.
                 | _ => L.2
                 end
       in match a, L1 with
-         | a_send p, l_send q ty L' =>
-           if (p.1.2 == q) && (p.2 == ty) then Some L'
-           else None
-         | a_recv p, l_recv q ty L' =>
-           if (p.1.1 == q) && (p.2 == ty) then Some L'
-           else None
-         | a_brn p q lb, l_brn q' K =>
+         | a_send p q lb t, l_msg l_send q' K =>
            if q == q'
-           then lookup lb K
+           then match lookup lb K with
+                | Some (t', s) => if t == t' then Some s else None
+                | None => None
+                end
            else None
-         | a_sel p q lb, l_sel p' K =>
-           if p == p'
-           then lookup lb K
+         | a_recv p q lb t, l_msg l_recv q' K =>
+           if q == q'
+           then match lookup lb K with
+                | Some (t', s) => if t == t' then Some s else None
+                | None => None
+                end
            else None
          | _, _ => None
          end
@@ -681,22 +565,14 @@ Section Semantics.
   Definition enqueue_lbl (Q : MsgQ) p q lb := enqueue Q ((p, q), inl lb) .
   (** lstep a Q P Q' P' is the 'step' relation <Q, P> ->^a <Q', P'> in Coq*)
   Inductive lstep : act -> MsgQ * PEnv -> MsgQ * PEnv -> Prop :=
-  | ls_snd p P Q P' Q' :
-      Q' == enqueue_msg Q p ->
-      Some P' == do_act (a_send p) P ->
-      lstep (a_send p) (Q, P) (Q', P')
-  | ls_rcv p P Q P' Q' :
-      Some (inr p.2, Q') == dequeue Q p.1 ->
-      Some P' == do_act (a_recv p) P ->
-      lstep (a_recv p) (Q, P) (Q', P')
-  | ls_sel p q lb P Q P' Q' :
+  | ls_send t p q lb P Q P' Q' :
       Q' == enqueue_lbl Q p q lb ->
-      Some P' == do_act (a_sel p q lb) P ->
-      lstep (a_sel p q lb) (Q, P) (Q', P')
-  | ls_brn p q lb P Q P' Q' :
+      Some P' == do_act (a_send p q lb t) P ->
+      lstep (a_send p q lb t) (Q, P) (Q', P')
+  | ls_recv t p q lb P Q P' Q' :
       Some (inl lb, Q') == dequeue Q (p, q) ->
-      Some P' == do_act (a_sel p q lb) P ->
-      lstep (a_brn p q lb) (Q, P) (Q', P')
+      Some P' == do_act (a_recv p q lb t) P ->
+      lstep (a_recv p q lb t) (Q, P) (Q', P')
   .
 
   CoInductive l_lts : trace -> MsgQ * PEnv -> Prop :=
